src/StandardLibrary/Consumers.dfy
@@ -1,0 +1,141 @@
+include "../StandardLibrary/StandardLibrary.dfy"
+include "../StandardLibrary/UInt.dfy"
+
+module Consumers {
+  import opened StandardLibrary
+  import opened UInt = StandardLibrary.UInt
+
+  trait ByteConsumer {
+    ghost const Repr: set<object>
+    predicate Valid() reads this, Repr ensures Valid() ==> this in Repr
+    predicate method CanAccept() reads this, Repr
+      requires Valid()
+      ensures Valid()
+    method Accept(b: uint8)
+      requires Valid()
+      requires CanAccept()
+      ensures Valid()
+      modifies this, Repr
+      decreases Repr
+  }
+
+  trait {:extern} ExternalByteConsumer {
+    ghost const Repr: set<object>
+    predicate method CanAccept() reads this, Repr decreases Repr
+    method Accept(b: uint8) modifies this, Repr decreases Repr
+  }
+
+  class AsExternalByteConsumer extends ExternalByteConsumer {
+    const wrapped: ByteConsumer
+    constructor(wrapped: ByteConsumer) {
+      this.wrapped := wrapped;
+      this.Repr := {this, wrapped} + wrapped.Repr;
+    }
+    predicate Valid() reads this, Repr ensures Valid() ==> this in Repr {
+      && this in Repr 
+      && wrapped in Repr 
+      && wrapped.Repr < Repr 
+      && this !in wrapped.Repr
+      && wrapped.Valid()
+    }
+    lemma {:axiom} AssumedValid() ensures Valid()
+    predicate method CanAccept() reads this, Repr decreases Repr {
+      AssumedValid();
+      wrapped.CanAccept()
+    }
+    method Accept(b: uint8) modifies this, Repr decreases Repr {
+      AssumedValid();
+      expect CanAccept();
+      wrapped.Accept(b);
+    }
+  }
+
+  class AsByteConsumer extends ByteConsumer {
+    const wrapped: ExternalByteConsumer
+    constructor(wrapped: ExternalByteConsumer) ensures Valid() {
+      this.wrapped := wrapped;
+      this.Repr := {this, wrapped} + wrapped.Repr;
+    }
+    predicate Valid() reads this, Repr ensures Valid() ==> this in Repr {
+      && this in Repr 
+      && wrapped in Repr 
+      && wrapped.Repr < Repr 
+      && this !in wrapped.Repr
+    }
+    predicate method CanAccept() reads this, Repr
+      requires Valid()
+      ensures Valid()
+      decreases Repr
+    {
+      wrapped.CanAccept()
+    }
+    method Accept(b: uint8) 
+      requires Valid()
+      ensures Valid()
+      modifies this, Repr
+      decreases Repr
+    {
+      wrapped.Accept(b);
+    }
+  }
+
+  method ToExternalByteConsumer(c: ByteConsumer) returns (res: ExternalByteConsumer)
+  {
+    var result := Cast<AsByteConsumer>(c, _ => true);
+    match result {
+      case Some(adaptor) => 
+        res := adaptor.wrapped; 
+      case None =>
+        res := new AsExternalByteConsumer(c);
+    }
+  }
+
+  method FromExternalByteConsumer(c: ExternalByteConsumer) returns (res: ByteConsumer) 
+    ensures res.Valid()
+  {
+    var result := Cast<AsExternalByteConsumer>(c, _ => true);
+    match result {
+      case Some(adaptor) =>
+        adaptor.AssumedValid();
+        res := adaptor.wrapped; 
+      case None =>
+        res := new AsByteConsumer(c);
+    }
+  }
+
+  class ArrayWritingByteConsumer extends ByteConsumer {
+    const bytes: array<uint8>
+    var index: int
+    var maxIndex: int
+    predicate Valid() reads this {
+      && 0 <= index <= maxIndex <= bytes.Length
+      && Repr == {this, bytes}
+    }
+    constructor(bytes: array<uint8>) 
+      ensures Valid()
+      ensures fresh(Repr - {this, bytes})
+    {
+      this.bytes := bytes;
+      this.index := 0;
+      this.maxIndex := bytes.Length;
+      this.Repr := {this, bytes};
+    }
+    predicate method CanAccept() reads this requires Valid() ensures Valid() {
+      index < maxIndex
+    }
+    method Accept(b: uint8)
+      requires Valid()
+      requires CanAccept()
+      ensures Valid()
+      modifies Repr
+      decreases Repr
+    {
+      bytes[index] := b;
+      index := index + 1;
+    }
+
+    function method Capacity(): nat reads this requires Valid() {
+      maxIndex - index
+    }
+  }
+}
